Members included from different files are now internally marked with an IncludeToken; the previous scheme of using {:verify false} is no longer used.  This makes "include" work with refinement features. Filenames of included files used in error messages are now what the user wrote, rather than absolute paths (which not only don't look so good, but are also problematic in comparing test output on different machines). Added dafny0/Includee.dfy to the test suite as well -- might as well include it, too, to get checked.

Source/Dafny/DafnyAst.cs
@@ -49,17 +49,20 @@ namespace Microsoft.Dafny {
   public class Include : IComparable
   {
     public readonly IToken tok;
-    public readonly string filename;    
+    public readonly string filename;
+    public readonly string fullPath;
 
-    public Include(IToken tok, string theFilename) {
+    public Include(IToken tok, string theFilename, string fullPath) {
       this.tok = tok;
-      this.filename = theFilename;      
+      this.filename = theFilename;
+      this.fullPath = fullPath;
     }
 
 
     public int CompareTo(object obj) {
-      if (obj is Include) {
-        return this.filename.CompareTo(((Include)obj).filename);
+      var i = obj as Include;
+      if (i != null) {
+        return this.fullPath.CompareTo(i.fullPath);
       } else {
         throw new NotImplementedException();
       }
@@ -3962,6 +3965,19 @@ namespace Microsoft.Dafny {
     }
     public IToken Outer { get { return WrappedToken; } }
     public readonly IToken Inner;
+  }
+
+  /// <summary>
+  /// An IncludeToken is a wrapper that indicates that the function/method was
+  /// declared in a file that was included. Any proof obligations from such an
+  /// included file are to be ignored.
+  /// </summary>
+  public class IncludeToken : TokenWrapper
+  {
+    public IncludeToken(IToken wrappedToken)
+      : base(wrappedToken) {
+      Contract.Requires(wrappedToken != null);
+    }
   }
 
   // ------------------------------------------------------------------------------------------------------
