Test/dafny0/Includee.dfy
@@ -1,10 +1,26 @@
 
 method m_unproven(x:int) returns (y:int)
   ensures y == 2*x;
-{
+{  // error: postcondition violation
 }
 
 function f(x:int) : int
 {
   2*x
+}
+
+abstract module Abstract
+{
+  function method inc(x:int) :int
+    ensures inc(x) > x;
+
+  method M(x: int) returns (r: int)
+    ensures r == x;
+  {  // error: postcondition violation
+    var y :| 0 <= y;
+    r := x + 3;
+    assert r % 3 == 0;  // error
+  }
+
+  function method G(x: int): int
 }
